theories/valid_tree_subst.v
@@ -4,39 +4,36 @@ From det Require Import lang ctx.
 From det Require Import tree tree_prop unif.
 
 (* valid_tree_subst *)
-Fixpoint vts s A :=
+Fixpoint vts_aux s A :=
+  let vts_aux := vts_aux s in
   match A with
-  | TA _ | OK | KO => true
-  | Or None sm B => [&& mp s sm & vts s B]
-  | Or (Some A) sm B => 
-      [&& mp s sm, vts s A & vts s B]
-  | And A B0 B => vts s A && vts s B
+  | Unexplored _ | OK | KO => true
+  | Or None sm B => [&& mp s sm & vts_aux B]
+  | Or (Some A) sm B => [&& mp s sm, vts_aux A & vts_aux B]
+  | And A B0 B => vts_aux A && vts_aux B
   end.
 
+Fixpoint vts s A :=
+  match A with
+  | Unexplored _ | OK | KO => true
+  | Or None sm B => vts sm B
+  | Or (Some A) sm B => [&& vts_aux s A, vts s A & vts sm B]
+  | And A B0 B => [&& vts_aux s A, vts_aux s B, vts s A & vts s B]
+  end.
+
+Lemma vts_aux_big_andA s x xs: vts_aux s (big_andA x xs).
+Proof. by elim: xs x => //=. Qed.
+
+Lemma vts_aux_big_and s xs: vts_aux s (big_and xs).
+Proof. case: xs => //= ??; apply: vts_aux_big_andA. Qed.
+
 Lemma vts_big_and s l : vts s (big_and l).
-Proof. case: l => //=x xs; elim: xs x => //=. Qed.
+Proof. by case: l => //= x xs; elim: xs x => //=x xs ->; rewrite vts_aux_big_andA. Qed.
 
 Definition all_mp T sm (l: seq (_ * T)) := all (mp sm) (map fst l).
 
 Lemma all_mp_cons T s x xs: @all_mp T s (x :: xs) = mp s x.1 && all_mp s xs.
 Proof. by []. Qed.
-
-Lemma vts_big_or s a l : all_mp s l -> vts s (big_or a l).
-Proof.
-  elim: l a => //= [|[s' x] xs IH] a H; first by apply: vts_big_and.
-  move: H; rewrite all_mp_cons => /andP[H1 H2]/=.
-  by rewrite IH//vts_big_and H1.
-Qed.
-
-Lemma vt_cut {A} s: vts s A -> vts s (cutl A).
-Proof.
-  elim_tree A s => /=.
-    by move=> /and3P[H1 H2 H3]; rewrite H1 HA.
-    by move=> /andP[H1 H2]; rewrite H1 HB.
-  by move=> /andP[H1 H2]; case: ifP => //=; rewrite HA//HB//.
-Qed.
-
-Definition u := mk_Unif unify matching.
 
 Lemma mp_trans: transitive mp.
 Proof.
@@ -47,26 +44,88 @@ Proof.
   rewrite derefxx//.
 Qed.
 
-Lemma mp_H f m l1 l2 s s':
-  acyclic_sigma s -> H u f m l1 l2 s = Some s' -> mp s s'.
+Lemma mp_vts_aux o n t: mp o n -> vts_aux n t -> vts_aux o t.
 Proof.
-  elim: m l1 l2 s => [|x xs IH][|l1 l1s][|l2 l2s]//=s A.
-    by move=> [<-]; apply: mp_id.
-  case M: (_ l2) => [s2|]//= H.
-  have D: disjoint_L s [:: (deref s l2, deref s l1)].
-    by rewrite disjoint_L_cons !acyclic_deref_disjoint// disjoint_L0.
-  suffices [A' M'] : acyclic_sigma s2 /\ mp s s2.
-    by apply/mp_trans/IH/H.
-  by move: M; case: x => //= M; have -> := matching_acyclic A M;
-  have := montanari_mp A D M.
+  move=> MP; elim_tree t => //=.
+    by move=> /and3P[/(mp_trans MP)->/HA->/HB->].
+    by move=> /andP[/(mp_trans MP)->/HB->].
+  by move=> /andP[/HA->].
 Qed.
 
-Lemma all_mp_select pred args modes rules s r: acyclic_sigma s ->
-  select u pred args modes rules s = r -> all_mp s r.2.
+Lemma mp_vts o n t: mp o n -> vts n t -> vts o t.
 Proof.
-  move=> A <-; elim: rules => //= r0 rs IH.
-  case: ifP => _ //=; case H: H => [s'|]//.
-  rewrite//push/=all_mp_cons/= IH andbT.
+  move=> MP; elim_tree t => //=.
+    by move=> /and3P[/mp_vts_aux->///HA->->].
+  by move=> /and4P[/mp_vts_aux->///mp_vts_aux->///HA->/HB->].
+Qed.
+
+Lemma all_mp_trans {T} o n t: mp o n -> @all_mp T n t -> all_mp o t.
+Proof. by move=> mon H; apply/allP => x xH; have:= allP H x xH; apply/mp_trans. Qed.
+
+Lemma vts_aux_big_or o a l : all_mp o l -> vts_aux o (big_or a l).
+Proof.
+  elim: l o a => //= [|[n x] xs IH] o a; first by rewrite vts_aux_big_and.
+  by rewrite all_mp_cons => /=/andP[mp/IH->]; rewrite mp vts_aux_big_and.
+Qed.
+
+
+Lemma vts_big_or o a l : vts o (big_or a l).
+Proof.
+  elim: l o a => //= [|[n x] xs IH] o a; first by rewrite vts_big_and.
+  rewrite //=vts_big_and vts_aux_big_and/= IH//.
+Qed.
+
+Lemma vt_aux_cut {A} s: vts_aux s A -> vts_aux s (cutl A).
+Proof.
+  elim_tree A s => /=.
+    by move=> /and3P[H1 H2 H3]; rewrite H1 HA.
+    by move=> /andP[H1 H2]; rewrite H1 HB.
+  by move=> /andP[H1 H2]; case: ifP => //=; rewrite HA//HB//.
+Qed.
+
+Lemma vt_cut {A} s: vts s A -> vts s (cutl A).
+Proof.
+  elim_tree A s => //=.
+    by move=> /and3P[H1 H2 H3]; rewrite HA//vt_aux_cut.
+    by apply: HB.
+  by move=> /and4P[H1 H2 H3 H4]; case: ifP; rewrite//=!vt_aux_cut//HA//HB.
+Qed.
+
+Definition u := mk_Unif unify matching.
+
+(* TODO: already in mut_excl *)
+Lemma acyclic_sigma_H sP fv q hd s1 r:
+  acyclic s1 -> H u sP fv q hd s1 = Some r -> acyclic r.2.
+Proof.
+  elim: q fv hd s1 r => //=[p|f Hf a Ha] fv [p'|//|f' a']// s1 r.
+    by case: eqP => //= _ A; case: fndP => //=pP[<-].
+  move=> A.
+  case H: H => [[[|[] tyl tyr] s1']|]//=.
+    case M: matching => //= [s1''][?]; subst.
+    by apply: matching_acyclic M; apply: Hf H.
+  case M: unify => //= [s1''][?]; subst.
+  by apply: unif_acyclic M; apply: Hf H.
+Qed.
+
+
+Lemma mp_H froz m l1 l2 s s':
+  acyclic s -> H u froz m l1 l2 s = Some s' -> mp s s'.2.
+Proof.
+  move=>As; elim: l1 s' l2 => //=[p|f Hf a Ha] s' [p'|v'|f' a']//=.
+    by case: eqP => //->; case: fndP => //= pf [<-]//=; rewrite mp_id.
+  case H: H => //[[[//|md tl tr] s'']].
+  case X: (_ a') => //=[sx][<-{s'}]/=.
+  apply: mp_trans (Hf _ _ H) _.
+  have /=As'' := acyclic_sigma_H As H.
+  have Hx := disjoint_L_deref _ _ As''.
+  case: md X {H} => //=; apply: montanari_mp => //=.
+Qed.
+
+Lemma all_mp_select sig t rules s: acyclic s ->
+  all_mp s (select u sig t rules s).
+Proof.
+  move=> A; elim: rules => //= r0 rs IH.
+  case H: H => [[ty s']|]//=; rewrite all_mp_cons IH andbT.
   by apply: mp_H H.
 Qed.
 
@@ -74,79 +133,117 @@ Lemma all_mp_bc p sv t s r:
   (bc u p sv t s) = r -> all_mp s r.2.
 Proof.
   move=> <-; rewrite/bc.
-  case (boolP (acyclic_sigma s)) => A//=.
-  set D := deref _ _; case X: get_tm_hd => [pred|]//=.
-  case: fndP => //=pp.
-  rewrite !push/=.
-  by apply: all_mp_select erefl.
+  case (boolP (acyclic s)) => A//=.
+  by rewrite !push/=; apply: all_mp_select.
 Qed.
 
-Lemma vt_step p o n sv A r: mp o n ->
-  vts n A -> step u p sv n A = r -> vts o r.2.
+Lemma mp_next_subst o A n: mp o n ->
+  vts_aux o A -> mp o (next_subst n A).
 Proof.
-  move=>++<-; clear r.
-  elim_tree A o n sv => /= mon.
-  + case: t => [|t]//=; rewrite push/=.
-    case B : bc => [sv' [|[x sx] xs]]/=//= _.
-    have:= all_mp_bc B; rewrite all_mp_cons/=.
-    move=> /andP[H /vts_big_or].
-    admit.
+  elim_tree A o n => mon/=.
+    by move=> /and3P[H1 H2 H3]; rewrite HA//.
+    by move=> /andP[H1 H2]; rewrite HB//.
+  move=> /andP[H1 H2]/=; rewrite next_subst_and.
+  by case: ifP => //; rewrite !(HA,HB)//.
+Qed.
+
+Lemma bc_mp_all p sv sv' t n l:
+  bc u p sv t n = (sv', l) ->
+  all_mp n l.
+Proof.
+  rewrite (surjective_pairing (bc _ _ _ _ _)) => -[_{sv'}<-{l}].
+  rewrite/bc; case: ifP => //= /negbFE A.
+  by rewrite !push/= all_mp_select.
+Qed.
+
+Lemma vts_aux_step p o n sv A: mp o n ->
+  vts_aux o A -> vts_aux o (step u p sv n A).2.
+Proof.
+  elim_tree A n o sv => //=mon.
+  + case: t => [|t]//=; rewrite push.
+    case B : bc => [sv' [|[x sx] xs]]//= _.
+    have:= bc_mp_all B; rewrite all_mp_cons.
+    move=> /andP[/(mp_trans mon)-> H].
+    by rewrite vts_aux_big_or//(all_mp_trans mon).
   + move=> /and3P[H vA vB]; set S:= step _ _ _ _ _.
-    have Hx : vts n (if is_cb S.1.2 then KO else B) by case: ifP.
-    rewrite !push/= HA//=. H Hx andbT/= /S.
-    apply: HA.
-    rewrite andbT/=.
-    app HA s sv; rewrite S.
-    apply: 
-    have:= HA _ sv vA.
-
-    case: bc => [_ []]//=. -[]//= _ >; rewrite valid_tree_big_or.
-  + move=> /andP[vA bB]; rewrite !push/= HA//=; case: ifP => //.
-  + by move=> vB; rewrite !push /=; apply: HB.
-  + move=> /andP[vA].
-    rewrite !push.
-    case: ifP => [sA vB /= | sA]/=.
-      have {HB} := HB (next_subst s A) sv vB.
-      case X: step => //[[?[]]C]/=vC; try by rewrite sA vA vC.
-      rewrite success_cut sA/= vC valid_tree_cut//.
-    move=> /eqP -> {B HB}.
-    have:= HA s sv vA.
-    case X: step => //[[sv' []]A']/=vA'; only 1-3: by rewrite eqxx vA' valid_tree_big_and if_same.
-    have [? sA']:= step_success X; subst.
-    congruence.
+    by rewrite !push/=HA//=H; case: ifP.
+  + by move=> /andP[mn vB]; rewrite !push/= mn/= HB//=.
+  + move=> /andP[va vb]; case: ifP => _; rewrite !push/=; last by rewrite HA.
+    apply/andP; split; first by case: ifP; rewrite//vt_aux_cut.
+    by rewrite HB//mp_next_subst.
 Qed.
 
-Lemma valid_tree_prune A R b: 
-  valid_tree A -> prune b A = Some R -> valid_tree R.
+Lemma vts_step p o n sv A: mp o n ->
+  vts o A -> vts o (step u p sv n A).2.
 Proof.
-  elim_tree A R b => /=.
+  elim_tree A o n sv => /=mon.
+  + case: t => [|t]//= _; rewrite push/=.
+    case B : bc => [sv' [|[x sx] xs]]//=.
+    by rewrite vts_big_or.
+  + move=> /and3P[H vA vB]; set S:= step _ _ _ _ _.
+    have Hx : vts sm (if is_cb S.1.2 then KO else B) by case: ifP.
+    by rewrite !push/= HA//= Hx vts_aux_step//.
+  + move=> mp; rewrite !push/= HB//.
+    admit.
+  + move=> /and4P[va vb van vbn].
+    rewrite !fun_if !push/= vbn vb HA//!(HB,vts_aux_step)// ?(mp_id,mp_next_subst)//.
+    rewrite !fun_if/= !vt_cut//!vt_aux_cut//= va van.
+    repeat case: ifP => //.
+Admitted.
+
+Lemma vts_aux_prune o A R b: 
+  vts_aux o A -> prune b A = Some R -> vts_aux o R.
+Proof.
+  elim_tree A R o b => /=.
   + by case: R => //=; case: b => //.
   + by case: t => [|c]//= _ [<-]//.
-  + move=> /andP[vA bB]; case nA: prune => [A'|]//=.
-      by move=> [<-]/=; rewrite (HA A' b)//.
-    case nB: prune => [B'|]//[<-]/=; apply/HB/nB.
-    by move: bB => /orP[/eqP->|/spec_base_or[?[?]]]//<-; apply: valid_tree_big_or.
-  + by move=> vB; case nB: prune => [B'|]//=[<-]/=; apply/HB/nB.
-  + move=>/andP[vA].
-    case: ifP => /=[sA vB|sA]; subst.
+  + move=> /and3P[mp vA bB]; case nA: prune => [A'|]//=.
+      by move=> [<-]/=; rewrite (HA A' _ b)//mp.
+    by case nB: prune => [B'|]//[<-]/=; rewrite (HB _ _ _ _ nB)// mp.
+  + by move=> /andP[mp vB]; case nB: prune => [B'|]//=[<-]/=; rewrite mp; apply/HB/nB.
+  + move=>/andP[vA vB].
+    case: ifP => /= _.
       case X: prune => [D|].
-        move=>[<-]/=; rewrite vA sA/= (HB _ _ vB X)//.
+        by move=>[<-]/=; rewrite vA /= (HB _ _ _ _ X)//.
       case Y: prune => //=[A'].
-      by move=> [<-]/=; rewrite (HA _ true)//= valid_tree_big_and eqxx !if_same.
-    move=> /eqP->{B HB}.
+      by move=> [<-]/=; rewrite (HA _ _ true)//= vts_aux_big_and//.
     case: ifP => fA; last first.
-      by move=> [<-]/=; rewrite vA sA eqxx.
+      by move=> [<-]/=; rewrite vA.
     case X: prune => [D|]//=.
-    by move=> [<-]/=; rewrite (HA _ false)//= eqxx valid_tree_big_and !if_same.
+    by move=> [<-]/=; rewrite (HA _ _ false)//= vts_aux_big_and.
+  Qed.
+  
+Lemma vts_prune o A R b: 
+  vts o A -> prune b A = Some R -> vts o R.
+Proof.
+  elim_tree A R o b => /=.
+  + by case: R => //=; case: b => //.
+  + by case: t => [|c]//= _ [<-]//.
+  + move=> /and3P[mp vA bB]; case nA: prune => [A'|]//=.
+      by move=> [<-]/=; rewrite (HA _ _ _ _ nA)//=bB andbT (vts_aux_prune _ nA).
+    by case nB: prune => [B'|]//[<-]/=; rewrite (HB _ _ _ _ nB)// mp.
+  + by move=> vb; case nB: prune => [B'|]//=[<-]/=; apply: HB nB.
+  + move=>/and4P[vAa vBa vA vB].
+    case: ifP => /= _.
+      case X: prune => [D|].
+        by move=>[<-]/=; rewrite vA /= (HB _ _ _ _ X)//vAa (vts_aux_prune _ X).
+      case Y: prune => //=[A'].
+      by move=> [<-]/=; rewrite (HA _ _ true)//= vts_aux_big_and// vts_big_and (vts_aux_prune _ Y).
+    case: ifP => fA; last first.
+      by move=> [<-]/=; rewrite vA vAa vBa.
+    case X: prune => [D|]//=.
+    by move=> [<-]/=; rewrite (HA _ _ false)//= vts_aux_big_and (vts_aux_prune _ X)//vts_big_and.
   Qed.
 
-Lemma valid_tree_run s1 fv A b fv' s R:
-  valid_tree A -> runT u p fv s1 A (Many s R) b fv' -> valid_tree R.
+Lemma valid_tree_run p s1 fv A b fv' s R: acyclic s1 ->
+  vts s1 A -> runT u p fv s1 A (Many s R) b fv' -> vts s1 R.
 Proof.
   remember (Many _ _) as S eqn:HS.
-  move=> + H.
-  elim_run H s R HS => vA.
-  + by move: HS => [??]; subst; apply: valid_tree_prune NS.
-  + by apply: IH (valid_tree_step vA eA).
-  + by apply: IH (valid_tree_prune vA nA).
+  move=> ++ H.
+  elim_run H s R HS => As1 vA.
+  + by move: HS => [??]; subst; apply: vts_prune NS.
+  + move: eA; rewrite (surjective_pairing (step _ _ _ _ _)) => -[].
+    rewrite (surjective_pairing (step _ _ _ _ _).1) => -[???]; subst.  
+    apply: IH (vts_step _ _ _ _); rewrite// mp_id//.
+  + by apply: IH (vts_prune vA nA).
 Qed.
